Examples/EdmondsKarp_Maxflow/FordFulkerson_Algo.thy
@@ -6,12 +6,181 @@ imports
   "../../Refine_Imperative_HOL/Sepref"
   "../../RefineMonadicVCG"
 begin
+
+(* TODO: MOVE *)
+
+text \<open>Select some value with given property, or \<open>None\<close> if there is none.\<close>  
+definition SELECT :: "('a \<Rightarrow> bool) \<Rightarrow> enat \<Rightarrow> 'a option nrest"
+  where "SELECT P tf \<equiv> if \<exists>x. P x then REST (emb (\<lambda>r. case r of Some p \<Rightarrow> P p | None \<Rightarrow> False) tf)
+               else REST [None \<mapsto> tf]"
+
+                    
+lemma inresT_SELECT_Some: "inresT (SELECT Q tt) (Some x) t' \<longleftrightarrow> (Q x  \<and> (t' \<le> tt))"
+  by(auto simp: inresT_def SELECT_def emb'_def) 
+
+lemma inresT_SELECT_None: "inresT (SELECT Q tt) None t' \<longleftrightarrow> (\<not>(\<exists>x. Q x) \<and> (t' \<le> tt))"
+  by(auto simp: inresT_def SELECT_def emb'_def) 
+
+lemma inresT_SELECT[refine_pw_simps]:
+ "inresT (SELECT Q tt) x t' \<longleftrightarrow> ((case x of None \<Rightarrow> \<not>(\<exists>x. Q x) | Some x \<Rightarrow> Q x)  \<and> (t' \<le> tt))"
+  by(auto simp: inresT_def SELECT_def emb'_def) 
+
+
+lemma nofailT_SELECT[refine_pw_simps]: "nofailT (SELECT Q tt)"
+  by(auto simp: nofailT_def SELECT_def)
+
+lemma s1: "SELECT P T \<le> (SELECT P T') \<longleftrightarrow> T \<le> T'"
+  apply(cases "\<exists>x. P x") 
+   apply(auto simp: pw_le_iff refine_pw_simps split: option.splits)
+  subgoal 
+    by (metis (full_types) enat_ord_code(3) enat_ord_simps(1) lessI not_infinity_eq not_le order_mono_setup.refl) 
+  subgoal 
+    by (metis (full_types) enat_ord_code(3) enat_ord_simps(1) lessI not_enat_eq not_le order_mono_setup.refl) 
+  done
+     
+lemma s2: "SELECT P T \<le> (SELECT P' T) \<longleftrightarrow> (
+    (Ex P' \<longrightarrow> Ex P)  \<and> (\<forall>x. P x \<longrightarrow> P' x)) "
+  apply(auto simp: pw_le_iff refine_pw_simps split: option.splits)
+  subgoal 
+    by (metis enat_ile linear)                                          
+  subgoal 
+    by (metis enat_ile linear) 
+  done
+ 
+lemma SELECT_refine:
+  assumes "\<And>x'. P' x' \<Longrightarrow> \<exists>x. P x"
+  assumes "\<And>x. P x \<Longrightarrow>   P' x"
+  assumes "T \<le> T'"
+  shows "SELECT P T \<le> (SELECT P' T')"
+proof -
+  have "SELECT P T \<le> SELECT P T'"
+    using s1 assms(3) by auto
+  also have "\<dots> \<le> SELECT P' T'"
+    unfolding s2 apply safe
+    using assms(1,2) by auto  
+  finally show ?thesis .
+qed
+
+
+lemma TTT_SELECT: 
+  assumes  
+    "\<forall>x. \<not> P x \<Longrightarrow> Some tt \<le> TTT Q (SPECT [None \<mapsto> tf])"
+  and p: "(\<And>x. P x \<Longrightarrow> Some tt \<le> TTT Q (SPECT [Some x \<mapsto> tf]))"
+   shows "Some tt \<le> TTT Q (SELECT P tf)"
+proof(cases "\<exists>x. P x")
+  case True
+  from p[unfolded T_pw mii_alt] have
+    p': "\<And>y x. P y \<Longrightarrow> Some tt \<le> mm2 (Q x)([Some y \<mapsto> tf] x)"
+    by auto
+
+  from True 
+  show ?thesis 
+    unfolding SELECT_def apply (auto simp: emb'_def split: if_splits)
+    apply(auto simp: T_pw) subgoal for x xa apply(cases xa)
+      apply (simp add: mii_alt)
+      apply (simp add: mii_alt) apply safe subgoal for a
+        using p'[of a xa] by auto
+      done
+    done
+next
+  case False
+  then show ?thesis 
+    unfolding SELECT_def apply (auto simp: emb'_def split: if_splits) using assms by auto
+qed 
+
+lemma progress_SELECT_iff: "progress (SELECT P T) \<longleftrightarrow> T > 0"
+  unfolding progress_def SELECT_def emb'_def by (auto split: option.splits)
+
+lemmas [progress_rules] = progress_SELECT_iff[THEN iffD2]
+
+
+
+lemma case_prod_refine:
+  fixes P Q :: "'a \<Rightarrow> 'b \<Rightarrow> 'c nrest"
+  assumes
+    "\<And>a b. P a b \<le> Q a b"
+  shows
+ "(case x of (a,b) \<Rightarrow> P a b) \<le> (case x of (a,b) \<Rightarrow> Q a b)"
+  using assms 
+  by (simp add: split_def)
+
+lemma case_option_refine:
+  fixes P Q :: "'a \<Rightarrow> 'b \<Rightarrow> 'c nrest"
+  assumes
+    "PN \<le> QN"
+    "\<And>a. PS a \<le> QS a"
+  shows
+ "(case x of None \<Rightarrow> PN | Some a \<Rightarrow> PS a ) \<le> (case x of None \<Rightarrow> QN | Some a \<Rightarrow> QS a )"
+  using assms 
+  by (auto split: option.splits)
+
+lemma ASSERT_refine: "(Q \<Longrightarrow> P) \<Longrightarrow> ASSERT P \<le> ASSERT Q"
+  by(auto simp: pw_le_iff refine_pw_simps)
+
+lemma ASSERT_leI: "\<Phi> \<Longrightarrow> (\<Phi> \<Longrightarrow> M \<le> M') \<Longrightarrow> ASSERT \<Phi> \<bind> (\<lambda>_. M) \<le> M'"
+  by(auto simp: pw_le_iff refine_pw_simps)
+
+lemma le_ASSERTI: "(\<Phi> \<Longrightarrow> M \<le> M') \<Longrightarrow> M \<le> ASSERT \<Phi> \<bind> (\<lambda>_. M')"
+  by(auto simp: pw_le_iff refine_pw_simps)
+
+lemma inresT_ASSERT: "inresT (ASSERT Q \<bind> (\<lambda>_. M)) x ta = (Q \<longrightarrow> inresT M x ta)"
+  unfolding ASSERT_def iASSERT_def by auto
+
+
+lemma nofailT_ASSERT_bind: "nofailT (ASSERT P \<bind> (\<lambda>_. M)) \<longleftrightarrow> (P \<and> nofailT M)"
+  by(auto simp: pw_bindT_nofailT pw_ASSERT)
+
+
+
+
 text \<open>In this theory, we formalize the abstract Ford-Fulkerson
   method, which is independent of how an augmenting path is chosen\<close>
 
+
+
+
+
+
+(*
+
+
+lemma (in FoFu) R_decreases:
+  assumes "NFlow c s t a"
+      "NPreflow.isAugmentingPath c s t a x"
+      "special_info c s t a x"
+  shows "R (NFlow.augment_with_path c a x) < R a"
+proof -
+  have 2: "Graph.isShortestPath (cf_of a) s x t"
+    using assms(3)  by simp
+
+  show "R (NFlow.augment_with_path c a x) < R a"
+  unfolding R_def  
+  using NFlow.shortest_path_decr_ek_measure[OF assms(1) 2] 
+    NFlow.augment_with_path_def[OF assms(1) ] by auto
+qed 
+
+*)
+
+text \<open>We specify augmentation of a flow along a path\<close>
+definition (in NFlow) "augment_with_path p \<equiv> augment (augmentingFlow p)"
+ 
+locale FoFu = Network c s t for c :: "'capacity::linordered_idom graph" and s t +
+  fixes  R :: "(nat \<times> nat \<Rightarrow> 'capacity) \<Rightarrow> nat"
+     and   find_augmenting_time :: "nat "
+     and special_info :: "(nat \<times> nat \<Rightarrow> 'capacity) \<Rightarrow> (nat \<times> nat) list \<Rightarrow> bool"
+   assumes ff: "NFlow c s t a \<Longrightarrow>
+ \<forall>x. \<not> special_info a x
+   \<Longrightarrow> NPreflow.isAugmentingPath c s t a x \<Longrightarrow> False"  
+
+  and R_decreases: "NFlow c s t a \<Longrightarrow> special_info a x \<Longrightarrow> R (NFlow.augment_with_path c a x) < R a"
+
+  and fat_g_0: "\<And>x. find_augmenting_time  > 0"
+
+  and augments: "\<And>p f.  NFlow c s t f \<Longrightarrow> special_info f p \<Longrightarrow> NPreflow.isAugmentingPath c s t f p"
+
+
 context Network 
 begin
-
 
 (*
 context
@@ -20,13 +189,13 @@ context
 begin
 *)
 (* some measure that decreases after each loop of the edmondsKarp algorithm  
-  ek_analysis_defs.ekMeasure is a possible? *)
+  ek_analysis_defs.ekMeasure is a possible?  
 definition R :: "(nat \<times> nat \<Rightarrow> 'capacity) \<Rightarrow> nat" where 
   "R cf = ek_analysis_defs.ekMeasure (residualGraph c cf) s t"
 
 (* upper bound on the runtime of the algorithm for finding an
-    augmenting path *)
-definition find_augmenting_time :: "(nat \<times> nat \<Rightarrow> 'capacity) \<Rightarrow> nat " where
+    augmenting path
+definition  where
   "find_augmenting_time f = 10"
 
 definition "special_info f p \<equiv> Graph.isShortestPath (cf_of f) s p t"
@@ -36,12 +205,7 @@ lemma ff: "NFlow c s t a \<Longrightarrow>
    \<Longrightarrow> NPreflow.isAugmentingPath c s t a x \<Longrightarrow> False"  
   using NFlow.augmenting_path_imp_shortest NFlow.shortest_is_augmenting special_info_def by blast
   
-
-
-text \<open>Select some value with given property, or \<open>None\<close> if there is none.\<close>  
-definition SELECT :: "('a \<Rightarrow> bool) \<Rightarrow> enat \<Rightarrow> 'a option nrest"
-  where "SELECT P tf \<equiv> if \<exists>x. P x then REST (emb (\<lambda>r. case r of Some p \<Rightarrow> P p | None \<Rightarrow> False) tf)
-               else REST [None \<mapsto> tf]"
+ *) *)
 
 subsection \<open>Algorithm\<close>
 text \<open>
@@ -49,29 +213,13 @@ text \<open>
   Assuming a valid flow, the procedure must return an augmenting path 
   iff there exists one.
   \<close>
-definition "find_augmenting_spec f \<equiv> do {
+definition (in FoFu) "find_augmenting_spec f \<equiv> do {
     ASSERT (NFlow c s t f);
-    SELECT (%p. NPreflow.isAugmentingPath c s t f p \<and> special_info f p) (find_augmenting_time f)
+    SELECT (%p. (* NPreflow.isAugmentingPath c s t f p \<and> *) special_info f p) (find_augmenting_time)
   }"
 
-text \<open>Moreover, we specify augmentation of a flow along a path\<close>
-definition (in NFlow) "augment_with_path p \<equiv> augment (augmentingFlow p)"
- 
 
-lemma R_decreases:
-  assumes "NFlow c s t a"
-      "NPreflow.isAugmentingPath c s t a x"
-      "special_info a x"
-  shows "R (NFlow.augment_with_path c a x) < R a"
-proof -
-  have 2: "Graph.isShortestPath (cf_of a) s x t"
-    using assms(3) special_info_def by simp
 
-  show "R (NFlow.augment_with_path c a x) < R a"
-  unfolding R_def  
-  using NFlow.shortest_path_decr_ek_measure[OF assms(1) 2] 
-    NFlow.augment_with_path_def[OF assms(1) ] by auto
-qed
     
 
 text \<open>
@@ -84,7 +232,7 @@ abbreviation "fofu_invar \<equiv> \<lambda>(f,brk).
 
 text \<open>Finally, we obtain the Ford-Fulkerson algorithm.
   Note that we annotate some assertions to ease later refinement\<close>
-definition "fofu \<equiv> do {
+definition (in FoFu) "fofu \<equiv> do {
   f\<^sub>0 \<leftarrow> RETURNT (\<lambda>_. 0);
 
   (f,_) \<leftarrow> whileT(*\<^bsup>fofu_invar\<^esup>*)
@@ -137,47 +285,13 @@ lemma (in NFlow) augmenting_path_not_empty:
 text \<open>Finally, we can use the verification condition generator to
   show correctness\<close>
 
-fun Te where "Te (f,brk) = (if brk then 0 else find_augmenting_time f * (1+ R f))"
+fun (in FoFu) Te where "Te (f,brk) = (if brk then 0 else find_augmenting_time  * (1+ R f))"
 
 
-definition "maxFlow_time = enat (find_augmenting_time (\<lambda>_. 0) * (R (\<lambda>_. 0)))"
-
-lemma TTT_SELECT: 
-  assumes  
-    "\<forall>x. \<not> P x \<Longrightarrow> Some tt \<le> TTT Q (SPECT [None \<mapsto> tf])"
-  and p: "(\<And>x. P x \<Longrightarrow> Some tt \<le> TTT Q (SPECT [Some x \<mapsto> tf]))"
-   shows "Some tt \<le> TTT Q (SELECT P tf)"
-proof(cases "\<exists>x. P x")
-  case True
-  from p[unfolded T_pw mii_alt] have
-    p': "\<And>y x. P y \<Longrightarrow> Some tt \<le> mm2 (Q x)([Some y \<mapsto> tf] x)"
-    by auto
-
-  from True 
-  show ?thesis 
-    unfolding SELECT_def apply (auto simp: emb'_def split: if_splits)
-    apply(auto simp: T_pw) subgoal for x xa apply(cases xa)
-      apply (simp add: mii_alt)
-      apply (simp add: mii_alt) apply safe subgoal for a
-        using p'[of a xa] by auto
-      done
-    done
-next
-  case False
-  then show ?thesis 
-    unfolding SELECT_def apply (auto simp: emb'_def split: if_splits) using assms by auto
-qed 
+definition (in FoFu) "maxFlow_time = enat (find_augmenting_time * (R (\<lambda>_. 0) + 1)) "
 
 
-thm NFlow.shortest_path_decr_ek_measure
-
-
-lemma progress_SELECT_iff: "progress (SELECT P T) \<longleftrightarrow> T > 0"
-  unfolding progress_def SELECT_def emb'_def by (auto split: option.splits)
-
-lemmas [progress_rules] = progress_SELECT_iff[THEN iffD2]
-
-theorem fofu_partial_correct: "fofu \<le> SPECT (emb (\<lambda>f. isMaxFlow f) (maxFlow_time))"
+theorem (in FoFu)  fofu_partial_correct: "fofu \<le> SPECT (emb (\<lambda>f. isMaxFlow f) (maxFlow_time))"
   unfolding fofu_def find_augmenting_spec_def 
   apply(rule T_specifies_I)
   apply (vcg'\<open>-\<close>)    
@@ -185,7 +299,7 @@ theorem fofu_partial_correct: "fofu \<le> SPECT (emb (\<lambda>f. isMaxFlow f) (
   apply (rule T_conseq4)
    apply (rule whileT_rule'''[OF refl, where I="(\<lambda>e. if fofu_invar e
                 then Some (Te e) else None)"])
-  subgoal (*progress*) by (progress'\<open>auto simp: find_augmenting_time_def zero_enat_def\<close>)   
+  subgoal (*progress*) by (progress'\<open>auto simp: fat_g_0 zero_enat_def\<close>)   
     apply (vcg'\<open>-\<close>)  apply(rule TTT_SELECT)   
   subgoal (* no augmenting path *)    
     apply (vcg'\<open>-\<close>) 
@@ -193,11 +307,12 @@ theorem fofu_partial_correct: "fofu \<le> SPECT (emb (\<lambda>f. isMaxFlow f) (
   subgoal for f brk p (* found augmenting path *)    
     apply (vcg'\<open>-\<close>)
     subgoal unfolding NFlow.augment_with_path_def
-      using  NFlow.augment_pres_nflow by metis
-    subgoal using NFlow.augmenting_path_not_empty by metis
-    subgoal  unfolding find_augmenting_time_def  
+      using  NFlow.augment_pres_nflow augments by metis
+    subgoal using NFlow.augmenting_path_not_empty augments  by metis
+    subgoal  using  augments by simp 
+    subgoal 
       by (simp add: R_decreases less_imp_le_nat)
-    subgoal unfolding find_augmenting_time_def   using R_decreases[of "f" "p"] by simp 
+    subgoal by (metis R_decreases diff_mult_distrib2 prod_ineqs2 zero_less_diff)
   done
   apply (auto simp: zero_flow)
   apply (vcg'\<open>-\<close>)
